Projects/AP/FreshA/Fresh.lean
@@ -1,5 +1,4 @@
 import Projects.AP.FreshA.Nbhd
-import Projects.Temp
 
 namespace AP
 
